PMapHelperLemmas.v
@@ -6,7 +6,7 @@ Transparent lookup_ctrl.
 Lemma commute_lookup_eval_ctrl:
   forall c f s,
   lookup_ctrl (eval_sym_state s f) c =
-  eval_smt_arith (lookup_ctrl s c) f.
+  Initialized uint8 (eval_smt_arith (lookup_ctrl s c) f).
 Proof.
   intros.
   apply PMap.gmap.
@@ -18,7 +18,7 @@ Transparent lookup_hdr_map.
 Lemma commute_lookup_eval_hdr:
   forall h f s,
   lookup_hdr (eval_sym_state s f) h =
-  eval_smt_arith (lookup_hdr s h) f.
+  Initialized uint8 (eval_smt_arith (lookup_hdr s h) f).
 Proof.
   intros.
   apply PMap.gmap.
@@ -29,7 +29,7 @@ Transparent lookup_state_map.
 Lemma commute_lookup_eval_state:
   forall sv f s,
   lookup_state (eval_sym_state s f) sv =
-  eval_smt_arith (lookup_state s sv) f.
+  Initialized uint8 (eval_smt_arith (lookup_state s sv) f).
 Proof.
   intros.
   apply PMap.gmap.
